SetoidGraphs/IndependentSets.v
@@ -5,24 +5,99 @@ Require Import MathClasses.implementations.list_finite_set
         MathClasses.orders.lattices
         MathClasses.orders.orders.
 Require Import MathClasses.interfaces.abstract_algebra.
+Require Import Bool.
 (*         MathClasses.interfaces.orders. *)
-Section IndependentSets.
-  Context `(GraphProperties).
+Set Implicit Arguments.
 
+Ltac solve_by_inverts n :=
+  try red;
+  match goal with | H : ?T |- _ => 
+  match type of T with Prop =>
+    solve [ 
+      inversion H; try reflexivity; eauto;
+      match n with S (S (?n')) => subst; solve_by_inverts (S n') end ]
+  end end.
+
+Ltac si :=
+  (intros; try setoid_discriminate; eauto; 
+  try match goal with
+      | H : _ /\ _ |- _ => intuition
+      | |- _ /\ _ => intuition
+      end;
+  intros; eauto;
+  try solve_by_inverts 4); eauto.
+
+Section IndependentSets.
+  Context `(Graph).
+  Definition asdf : Type.
+    
   Program  Definition IndependentSet (X : set_type vertex) (g : t) :=
     forall (x y : vertex),
       contains x X -> contains y X ->
       ~contains (buildEdge x y) (enumEdges g).
 
-  Context `(listset vertex).
-  Definition asdf : Type.
+  (* Context `(listset vertex). *)
+  (* Definition asdf : Type. *)
   
-Definition independentSet (X : set_type vertex) (g : t)
-    :=
-      fset_map id X.
+  Definition independentSet (X : set_type vertex) (G : t)
+    := for_all (fun v1 => for_all
+        (fun v2 => negb (mem (buildEdge v1 v2) (enumEdges G))) X) X.
   
+
+  Theorem independentSet_true_iff :
+    forall X G,
+  reflect (IndependentSet X G) (independentSet X G). 
+  Proof.
+    intros.
+    apply iff_reflect.
+    symmetry.
+    unfold independentSet, IndependentSet.
+    split; intros.
+    {
+      intros Hnot.
+      rewrite for_all_forall in H9.
+      apply H9 in H10.
+      rewrite for_all_forall in H10.
+      apply H10 in H11.
+      rewrite negb_true_iff in H11.
+      destruct (mem_reflect (buildEdge x y) (enumEdges G)); 
+      si.
+    }
+    repeat (rewrite for_all_forall; intros).
+    rewrite negb_true_iff.
+    destruct (mem_reflect (buildEdge v v0) (enumEdges G)); auto.
+    exfalso.
+    apply (H9 v v0); auto.
+  Qed.
+
   Definition ValidSet (X : set_type vertex) (G : t) :=
     forall (x : vertex) , contains x X -> contains x (enumVertices G).
+
+  Definition validSet (X : set_type vertex) (G : t) : bool :=
+    for_all (fun  x => if mem x X then mem x (enumVertices G) 
+            else true ) X.
+
+  Theorem validSet_true_iff :
+    forall X G, reflect (ValidSet X G) (validSet X G).
+  Proof.
+    intros.
+    apply iff_reflect.
+    symmetry.
+    unfold validSet, ValidSet.
+    rewrite for_all_forall.
+    split; intros; auto.
+    {
+      assert (x ∈ X) by auto.
+      rewrite mem_iff in H10; auto.
+      apply H9 in H11.
+      rewrite mem_iff; auto.
+      rewrite H10 in H11; auto.
+    }
+    assert (contains v X) by auto.
+    apply H9 in H10.
+    rewrite mem_iff in H10,H11; auto.
+    rewrite H11; auto.
+  Qed.
 
   Theorem validSetRecr : 
     forall x (X : set_type vertex) G,
@@ -30,7 +105,91 @@ Definition independentSet (X : set_type vertex) (g : t)
   Proof.
     red. intros.
     unfold ValidSet in *.
-    apply H4; auto.
+    apply H9; auto.
     rewrite fset_in_join.
     auto.
   Qed.
+
+
+  Inductive IndSet (X : set_type vertex) (G : t) :=
+  | defIndSet : ValidSet X G -> IndependentSet X G -> IndSet X G. 
+
+  Definition indSet (X : set_type vertex) (G : t) : bool :=
+    validSet X G && independentSet X G.
+
+  Theorem indSet_reflect : forall X G, reflect (IndSet X G) (indSet X G).
+  Proof.
+    intros.
+    apply iff_reflect.
+    unfold indSet.
+    assert (reflect (ValidSet X G) (validSet X G)).
+    apply validSet_true_iff.
+    split; try constructor; intuition.
+    destruct (independentSet_true_iff X G);
+      destruct (validSet_true_iff X G); auto;
+    inversion H10;
+    contradiction.
+    apply andb_true_iff in H10.
+    destruct H10.
+    destruct (validSet_true_iff X G); auto;
+    si.
+    destruct (independentSet_true_iff X G); auto.
+    apply andb_true_iff in H10.
+    si.
+  Qed.
+
+
+  Theorem nilIndSet : IndSet ⊥ empty.
+  Proof.
+     constructor; unfold IndependentSet;
+      try constructor; try intros x y H; unfold ValidSet; intros;
+      try apply fset_notin_empty in H9; 
+      try contradiction.    
+  Qed.
+
+  Theorem empty_IndSet_spec : forall G, IndSet bottom G.
+  Proof.
+    intros.
+    constructor.
+    unfold ValidSet.
+    intros.
+    apply fset_notin_empty in H9.
+    contradiction.
+    unfold IndependentSet.
+    intros.
+    apply fset_notin_empty in H9.
+    contradiction.
+  Qed.
+
+  Theorem nilIndSetAdd : forall x G, contains x (enumVertices G) ->
+                       IndSet (join {{x}} bottom) G.
+  Proof.
+    intros x G H10.
+    constructor.
+    {
+      unfold ValidSet.
+      intros.
+      rewrite fset_in_add in H9.
+      destruct H9.
+      rewrite H9;
+        auto.
+      apply fset_notin_empty in H9; contradiction.
+    }      
+    unfold IndependentSet.
+    intros.
+    intros Hnot.
+    rewrite fset_in_add in H9,H11.
+    destruct H9.
+    destruct H11.
+    subst.
+    admit.
+    (* eapply IsEdgeEnum  in Hnot; eauto. *)
+    (* rewrite H9 in Hnot. *)
+    (* apply edges_irreflexive in Hnot. *)
+    apply fset_notin_empty in H11; contradiction.
+    apply fset_notin_empty in H9; contradiction.
+  Admitted.
+
+
+
+
